src/TeX/EmitTeX.sml
@@ -293,6 +293,9 @@ local
      | "_"     => (token_string "Underscore",1)
      | "IN"    => (token_string "In",1)
      | "NOTIN" => (token_string "NotIn",1)
+     | "\226\134\146" => (token_string "Map", 1) (* → *)
+     | "\226\138\162" => (token_string "Turnstile", 2) (* ⊢ *)
+     | "\226\151\129" => (token_string "LOpenTri", 1) (* ◁ *)
      | _       => (String.translate char_map s,String.size s)
 in
   val emit_latex =
@@ -422,6 +425,9 @@ fun pp_type_as_tex ostrm ty =
      (type_pp.pp_type (Feedback.trace ("Unicode", 0) Parse.type_grammar ())
         emit_latex ostrm) ty;
 
+val print_thm_turnstile = ref true
+val _ = register_btrace ("EmitTeX: print thm turnstiles", print_thm_turnstile)
+
 fun pp_theorem_as_tex ostrm thm =
   if is_datatype_thm thm then
     pp_datatype_theorem emit_latex ostrm thm
@@ -430,8 +436,9 @@ fun pp_theorem_as_tex ostrm thm =
                PPBackEnd.with_ppstream emit_latex ostrm
     in
       begin_block Portable.INCONSISTENT 0;
-      PP.add_stringsz ostrm (token_string "Turnstile",2);
-      add_string " ";
+      if (!print_thm_turnstile) then
+        (PP.add_stringsz ostrm (token_string "Turnstile",2); add_string " ")
+      else ();
       pp_term_as_tex ostrm (concl thm);
       end_block ()
     end;
